src/Typing.v
@@ -1,11 +1,9 @@
-From MCore Require Import Syntax Env Tactics.
-From TLC Require Import LibString LibNat LibList LibSet.
-
-Open Scope nat_scope.
+From TLC Require Import LibString LibLN LibEnv.
+From MCore Require Import Syntax Tactics.
 
 Module Typing (P : PAT).
-  Module E := Env P.
-  Export E.
+  Module S := Syntax P.
+  Export S.
 
   Module Type PATCHECK.
     Parameter ok_pat : env -> pat -> type -> env -> Prop.
@@ -22,35 +20,38 @@ Module Typing (P : PAT).
     (*********************************)
 
     Definition ok_data (Gamma : env) (d : data) : Prop :=
-      forall (T : tname),
-        T \indom d ->
-        tname_in T (tnames Gamma) /\
-          forall (K : con),
-            K \in (d[T] : set con) ->
-                  exists d ty, con_in K d ty T (cons Gamma)
+      ok d /\
+      forall T cons,
+        binds T cons d ->
+        binds T BindTName Gamma /\
+          forall K,
+            K \in cons -> exists d ty, binds K (BindCon d ty T) Gamma
     .
 
     Inductive ok_kind : env -> kind -> Prop :=
-    | KiType' : forall {Gamma : env},
+    | TypeOk : forall {Gamma : env},
         ok_kind Gamma KiType
-    (* | KiData' : forall {Gamma : env} {d : data}, *)
+    (* | DataOk : forall {Gamma : env} {d : data}, *)
     (*     ok_data Gamma d -> *)
     (*     ok_kind Gamma (KiData d) *)
     .
     #[export]
      Hint Constructors ok_kind : mcore.
 
+    Reserved Notation "Gamma |= T ~:: k " (at level 50).
     Inductive ok_type : env -> type -> kind -> Prop :=
-    | TyFVar' : forall {Gamma : env} {tv : tvar} {k : kind},
-        tvar_in tv k Gamma ->
-        ok_type Gamma (TyFVar tv) k
-    | TyArr' : forall {Gamma : env} {ty1 ty2 : type},
-        ok_type Gamma ty1 KiType ->
-        ok_type Gamma ty2 KiType ->
-        ok_type Gamma (TyArr ty1 ty2) KiType
-    | TyAll' : forall {Gamma : env} {k : kind} {ty : type},
-        ok_type (BindTVar k :: Gamma) (ty_open ty 0 0) KiType ->
-        ok_type Gamma (TyAll k ty) KiType
+    | KVar : forall Gamma tv k,
+        binds tv (BindTVar k) Gamma ->
+        Gamma |= TyFVar tv ~:: k
+    | KArr : forall Gamma ty1 ty2,
+        Gamma |= ty1 ~:: KiType ->
+        Gamma |= ty2 ~:: KiType ->
+        Gamma |= TyArr ty1 ty2 ~:: KiType
+    | KAll : forall L Gamma k ty,
+        ok_kind Gamma k ->
+        (forall X, X \notin L ->
+                   (Gamma & X ~ BindTVar k) |= {0 ~> TyFVar X} ty ~:: KiType) ->
+        Gamma |= TyAll k ty ~:: KiType
     (* | TyProd' : forall {Gamma : env} {ty1 ty2 : type}, *)
     (*     ok_type Gamma ty1 KiType -> *)
     (*     ok_type Gamma ty2 KiType -> *)
@@ -71,57 +72,64 @@ Module Typing (P : PAT).
     (*     d2 \c d1 -> *)
     (*     (forall {T : tname}, d2[T] \c d1[T]) -> *)
     (*     ok_type Gamma ty (KiData d2) *)
+    where " Gamma |= T ~:: k " := (ok_type Gamma T k)
     .
     #[export]
      Hint Constructors ok_type : mcore.
 
     Inductive ok_env : env -> Prop :=
-    | EnvEmpty : ok_env empty_env
-    | EnvTName : forall Gamma, ok_env Gamma -> ok_env (BindTName :: Gamma)
+    | EnvEmpty : ok_env empty
+    | EnvTName : forall Gamma X, ok_env Gamma -> X # Gamma -> ok_env (Gamma & X ~ BindTName)
     | EnvCon   :
-      forall Gamma d ty T,
+      forall Gamma K d ty T,
         ok_env Gamma ->
+        K # Gamma ->
         ok_data Gamma d ->
-        ok_type Gamma ty KiType ->
-        tname_in T (tnames Gamma) ->
-        ok_env (BindCon d ty T :: Gamma)
-    | EnvTVar : forall Gamma k,
+        Gamma |= ty ~:: KiType ->
+        binds T BindTName Gamma ->
+        ok_env (Gamma & K ~ BindCon d ty T)
+    | EnvTVar : forall Gamma X k,
         ok_env Gamma ->
+        X # Gamma ->
         ok_kind Gamma k ->
-        ok_env (BindTVar k :: Gamma)
-    | EnvVar : forall Gamma ty,
+        ok_env (Gamma & X ~ BindTVar k)
+    | EnvVar : forall Gamma x ty,
         ok_env Gamma ->
-        ok_type Gamma ty KiType ->
-        ok_env (BindVar ty :: Gamma)
-    | EnvMatch : forall Gamma m,
+        x # Gamma ->
+        Gamma |= ty ~:: KiType ->
+        ok_env (Gamma & x ~ BindVar ty)
+    | EnvMatch : forall Gamma M m,
         ok_env Gamma ->
-        ok_env (BindMatch m :: Gamma)
+        M # Gamma ->
+        ok_env (Gamma & M ~ BindMatch m)
     .
     #[export]
      Hint Constructors ok_env : mcore.
 
+    Reserved Notation "Gamma |= t ~: T " (at level 50).
     Inductive ok_term : env -> term -> type -> Prop :=
-    | TmFVar' : forall {Gamma : env} {x : var} {ty : type},
+    | TVar : forall Gamma x ty,
         ok_env Gamma ->
-        var_in x ty Gamma ->
-        ok_term Gamma (TmFVar x) ty
-    | TmLam' : forall {Gamma : env} {ty1 ty2 : type} {t : term},
-        ok_type Gamma ty1 KiType ->
-        ok_term (BindVar ty1 :: Gamma) (tm_open t 0 0) ty2 ->
-        ok_term Gamma (TmLam ty1 t) (TyArr ty1 ty2)
-    | TmApp' : forall {Gamma : env} {ty1 ty2 : type} {t1 t2 : term},
-        ok_term Gamma t1 (TyArr ty1 ty2) ->
-        ok_term Gamma t2 ty1 ->
-        ok_term Gamma (TmApp t1 t2) ty2
-    | TmTyLam' : forall {Gamma : env} {k : kind} {ty : type} {t : term},
+        binds x (BindVar ty) Gamma ->
+        Gamma |= TmFVar x ~: ty
+    | TLam : forall L Gamma ty1 ty2 t,
+        Gamma |= ty1 ~:: KiType ->
+        (forall x, x \notin L ->
+                   (Gamma & x ~ BindVar ty1) |= [0 ~> TmFVar x]t ~: ty2) ->
+        Gamma |= TmLam ty1 t ~: TyArr ty1 ty2
+    | TApp : forall Gamma ty1 ty2 t1 t2,
+        Gamma |= t1 ~: TyArr ty1 ty2 ->
+        Gamma |= t2 ~: ty1 ->
+        Gamma |= TmApp t1 t2 ~: ty2
+    | TTyLam : forall L Gamma k ty t,
         ok_kind Gamma k ->
-        ok_term (BindTVar k :: freshen_after Gamma)
-                (tm_ty_open t 0 0) (ty_open ty 0 0) ->
-        ok_term Gamma (TmTyLam k t) (TyAll k ty)
-    | TmTyApp' : forall {Gamma : env} {k : kind} {ty1 ty2 : type} {t : term},
-        ok_term Gamma t (TyAll k ty1) ->
-        ok_type Gamma ty2 k ->
-        ok_term Gamma (TmTyApp t ty2) (ty_bsubst ty1 0 ty2)
+        (forall X, X \notin L ->
+                   (Gamma & X ~ BindTVar k) |= [{0 ~> TyFVar X}]t ~: ({0 ~> TyFVar X}ty)) ->
+        Gamma |= TmTyLam k t ~: (TyAll k ty)
+    | TTyApp : forall Gamma k ty1 ty2 t,
+        Gamma |= t ~: TyAll k ty1 ->
+        Gamma |= ty2 ~:: k ->
+        Gamma |= TmTyApp t ty2 ~: ({0 ~> ty2}ty1)
     (* | TmFix' : forall {Gamma : env} {ty : type} {t : term}, *)
     (*     ok_term Gamma t (TyArr ty ty) -> *)
     (*     ok_term Gamma (TmFix t) ty *)
@@ -193,7 +201,7 @@ Module Typing (P : PAT).
     (*     ok_term Gamma t2 ty1 -> *)
     (*     pats_exhaustive ps ty1 -> *)
     (*     ok_term Gamma (TmSemApp t1 t2) ty2 *)
-    .
+    where " Gamma |= t ~: T " := (ok_term Gamma t T).
     #[export]
      Hint Constructors ok_term : mcore.
 
@@ -203,220 +211,51 @@ Module Typing (P : PAT).
     (**************************)
 
     Lemma ok_type_lct :
-      forall Gamma ty k,
-        ok_type Gamma ty k ->
-        ty_lc ty.
-    Proof. introv tykind. induction* tykind. Qed.
-    #[export]
-     Hint Resolve ok_type_lct : mcore.
+      forall Gamma T k,
+        Gamma |= T ~:: k ->
+        lct T.
+    Proof. introv Hk ; induction* Hk. Qed.
 
-    Lemma ok_env_type :
-      forall G1 G2 ty,
-        ok_env (G1 ++ BindVar ty :: G2) ->
-        ok_type G2 ty KiType.
-    Proof. introv Henv ; induction* G1 ; inverts* Henv. Qed.
-
-    Lemma ok_env_lct :
-      forall Gamma x ty,
+    Lemma ok_env_ok :
+      forall Gamma,
         ok_env Gamma ->
-        var_in x ty Gamma ->
-        ty_lc ty.
-    Proof.
-      introv Henv Hvar. unfolds vars.
-      forwards Hmem : Nth_mem Hvar.
-      forwards* [ Hmem' ? ] : mem_filter_inv Hmem.
-      forwards [ G1 (G2 & Heq) ] : mem_inv_middle Hmem' ; subst.
-      applys ok_type_lct.
-      applys* ok_env_type.
-    Qed.
+        ok Gamma.
+    Proof. introv Hwf ; induction* Hwf. Qed.
 
-    Lemma ok_term_lct :
-      forall Gamma t ty,
-        ok_term Gamma t ty ->
-        ty_lc ty.
-    Proof with eauto using ty_lc_fsubst with mcore.
-      introv ttype. induction* ttype.
-      { Case "TmVar". apply* ok_env_lct. }
-      { Case "TmApp". inverts* IHttype1. }
-      { Case "TmTyApp".
-        rewrite ty_bsubst_close_open with (x := 0).
-        inverts IHttype... }
-    Qed.
-    #[export]
-     Hint Resolve ok_term_lct : mcore.
-
-    Lemma ok_term_lc :
-      forall Gamma t ty,
-        ok_term Gamma t ty ->
-        tm_lc t.
-    Proof. introv ttype. induction* ttype. Qed.
-    #[export]
-     Hint Resolve ok_term_lc : mcore.
-
-    Lemma ok_data_weaken_var :
-      forall G1 G2 ty' d,
-        ok_data (G1 ++ G2) d ->
-        ok_data (G1 ++ BindVar ty' :: G2) d.
-    Proof. introv Hd. unfolds ok_data. rew_env* in *. Qed.
-
-    Lemma ok_kind_weaken_var :
-      forall G1 G2 ty' k,
-        ok_kind (G1 ++ G2) k ->
-        ok_kind (G1 ++ BindVar ty' :: G2) k.
+    Lemma ok_kind_weakening :
+      forall G3 G1 G2 k,
+        ok_kind (G1 & G3) k ->
+        ok_kind (G1 & G2 & G3) k.
     Proof. introv Hk. induction* Hk. Qed.
 
-    Lemma ok_kind_weaken_tvar :
-      forall G1 G2 k' k,
-        ok_kind (G1 ++ G2) k ->
-        ok_kind (G1 ++ BindTVar k' :: G2) k.
-    Proof. introv Hk. induction* Hk. Qed.
-
-    Lemma ok_type_weaken_var :
-      forall G1 G2 ty ty' k,
-        ok_type (G1 ++ G2) ty k ->
-        ok_type (G1 ++ BindVar ty' :: G2) ty k.
+    Lemma ok_type_weakening :
+      forall G3 G1 G2 T k,
+        ok_type (G1 & G3) T k ->
+        ok_env (G1 & G2 & G3) ->
+        ok_type (G1 & G2 & G3) T k.
     Proof.
-      introv Hty.
-      remember (G1 ++ G2) as Gamma eqn:HGamma.
-      gen G1.
-      induction Hty ; intros ; subst*.
-      { Case "TyFVar". constructor. unfolds tvar_in. rew_env* in *. }
-      { Case "TyAll". constructor. applys IHHty (BindTVar k :: G1). rew_list*. }
+      introv Hk Henv.
+      remember (G1 & G3) as Gamma. gen G3.
+      induction* Hk; intros; substs.
+      - constructors*. apply* binds_weaken.
+        apply* ok_env_ok.
+      - apply_fresh* KAll. apply* ok_kind_weakening.
+        apply_ih_bind* H1.
+        constructor*. apply* ok_kind_weakening.
     Qed.
 
-    Lemma ok_type_weaken_tvar :
-      forall G1 G2 x ty k' k,
-        x = length (tvars G1) ->
-        ok_type (G1 ++ G2) ty k ->
-        ok_type (freshen_before G1 ++ BindTVar k' :: freshen_after G2) (ty_freshen ty x) k.
+    Lemma ok_env_ok_type :
+      forall Gamma x T,
+        ok_env Gamma ->
+        binds x (BindVar T) Gamma ->
+        Gamma |= T ~:: KiType.
     Proof.
-      introv Heq Hty.
-      remember (G1 ++ G2) as Gamma eqn:HGamma.
-      gen G1 x.
-      induction Hty ; intros ; subst*.
-      { Case "TyFVar". unfold ty_freshen. simple_math. admit. admit. }
-      Admitted.
-
-    Lemma ok_term_weaken_var :
-      forall G1 G2 x t ty ty',
-        x = length (vars G1) ->
-        ok_term (G1 ++ G2) t ty ->
-        ok_env  (G1 ++ BindVar ty' :: G2) ->
-        ok_term (G1 ++ BindVar ty' :: G2) (tm_freshen t x) ty.
-    Proof with rew_env ; rew_list ; eauto using ok_kind_weaken_var, ok_type_weaken_var with mcore.
-    Admitted.
-    (*   introv Heq ttype. *)
-    (*   remember (G1 ++ G2) as Gamma eqn:HGamma. *)
-    (*   gen G1 x. *)
-    (*   induction ttype ; intros ; subst ; simpls... *)
-    (*   { Case "TmFVar". unfolds var_in. rew_env in *. *)
-    (*     forwards [ (Hlt & Hvar) | (Hge & Hvar) ] *)
-    (*       : binds_weaken ; simple_math ; constructor ; unfolds var_in... } *)
-    (*   { Case "TmLam". constructor... rewrite* tm_open_freshen_comm. *)
-    (*     applys IHttype (BindVar ty1 :: G1)... } *)
-    (*   { Case "TmTyLam". constructor... rewrite* tm_ty_open_freshen_comm. *)
-    (*     apply (IHttype (BindTVar k :: (map_vars (fun ty'0 => ty_freshen ty'0 0) G1)))... } *)
-    (* Qed. *)
-
-    (* Lemma ok_env_freshen : *)
-    (*   forall G1 G2 k, *)
-    (*     ok_env (G1 ++ G2) -> *)
-    (*     ok_kind G2 k -> *)
-    (*     ok_env (map_vars ty_freshen G1 ++ BindTVar k :: G2). *)
-    (* Proof. *)
-    (*   introv Henv Hk. *)
-    (*   induction G1. *)
-    (*   Admitted. *)
-    (*   { Case "nil". unfold env_freshen. rew_listx*. } *)
-    (*   { Case "cons". unfold env_freshen. rew_listx. } *)
-    (* Admitted. *)
-
-    Lemma ok_term_weaken_tvar :
-      forall G1 G2 x t ty k,
-        x = length (tvars G1) ->
-        ok_term (G1 ++ G2) t ty ->
-        ok_env  (freshen_before G1 ++ BindTVar k :: G2) ->
-        ok_term (freshen_before G1 ++ BindTVar k :: G2) (tm_ty_freshen t x) (ty_freshen ty x).
-    Proof with rew_env ; rew_list ; eauto using ok_kind_weaken_tvar, ok_type_weaken_tvar with mcore.
-      introv Heq ttype.
-      remember (G1 ++ G2) as Gamma eqn:HGamma.
-      gen G1 x.
-      induction ttype ; intros ; subst ; simpls*.
-      Admitted.
-      (* { Case "TmFVar". constructor*. unfolds var_in. rew_env in *... } *)
-      (* { Case "TmLam". constructor. unfolds var_in. rew_env in *... } *)
-
-    Lemma ok_data_strengthen_var :
-      forall G1 G2 ty' d,
-        ok_data (G1 ++ BindVar ty' :: G2) d ->
-        ok_data (G1 ++ G2) d.
-    Proof. introv Hd. unfolds ok_data. rew_env* in *. Qed.
-
-    Lemma ok_kind_strengthen_var :
-      forall G1 G2 ty' k,
-        ok_kind (G1 ++ BindVar ty' :: G2) k ->
-        ok_kind (G1 ++ G2) k.
-    Proof. introv Hk. induction* Hk. Qed.
-
-    Lemma ok_type_strengthen_var :
-      forall G1 G2 ty' ty k,
-        ok_type (G1 ++ BindVar ty' :: G2) ty k ->
-        ok_type (G1 ++ G2) ty k.
-    Proof.
-      introv Hty.
-      remember (G1 ++ BindVar ty' :: G2) as Gamma eqn:HGamma.
-      gen G1.
-      induction Hty ; intros ; subst*.
-      { Case "TyFVar". constructor. unfolds tvar_in. rew_env* in *. }
-      { Case "TyAll". constructor. applys IHHty (BindTVar k :: G1). rew_list*. }
+      introv Henv Hbind.
+      induction* Henv ; try (binds_cases Hbind ; apply_empty* ok_type_weakening).
+      - false. apply* binds_empty_inv.
+      - inverts* EQ.
     Qed.
 
-    Lemma ok_env_strengthen_var :
-      forall G1 G2 ty,
-        ok_env (G1 ++ BindVar ty :: G2) ->
-        ok_env (G1 ++ G2).
-    Proof with eauto using ok_data_strengthen_var, ok_kind_strengthen_var, ok_type_strengthen_var.
-      introv Henv ; induction* G1 ; rew_list in * ; inverts* Henv ; constructor ; rew_env in *...
-    Qed.
-
-    Lemma ok_term_ok_env :
-      forall Gamma t ty,
-        ok_term Gamma t ty ->
-        ok_env Gamma.
-    Proof. introv ttype ; induction* ttype ; inverts* IHttype. Admitted.
-
-    Lemma tm_close_preservation :
-      forall G1 G2 x t t' ty1 ty2,
-        x = length (vars G1) ->
-        ok_term (G1 ++ BindVar ty1 :: G2) t ty2 ->
-        ok_term (G1 ++ G2) t' ty1 ->
-        ok_term (G1 ++ G2) (tm_close t x t') ty2.
-    Proof with rew_env ; rew_list
-      ; eauto using ok_term_ok_env, ok_kind_strengthen_var, ok_type_strengthen_var, ok_env_strengthen_var
-        with mcore.
-      introv Heq ttype. unfolds tm_close.
-      remember (G1 ++ BindVar ty1 :: G2) as Gamma eqn:HGamma.
-      gen ty1 t' G1 x.
-      induction ttype ; intros ; subst ; simpls...
-      { Case "TmFVar". unfolds var_in. rew_env in *.
-        forwards [ (Hlt & Hvar') | [ (Heq1 & Heq2) | (Hgt & Hvar') ] ]
-          : binds_app_middle_inv ; subst ; simple_math ; try (constructor ; unfolds var_in)...
-        inverts* Heq2. rewrite* tm_defreshen_freshen. }
-      { Case "TmLam". constructor... folds (tm_close t (length (vars G1)) t').
-        rewrite* tm_open_close_comm. applys IHttype (BindVar ty1 :: G1)...
-        applys_eq (ok_term_weaken_var empty_env)... }
-      { Case "TmTyLam". constructor... folds (tm_close t (length (vars G1)) t').
-        rewrite* tm_ty_open_close_comm. unfolds freshen_after. rew_listx in *.
-        apply (IHttype (ty_freshen ty1 0) (tm_ty_freshen t' 0) (BindTVar k :: freshen_after G1)).
-        applys_eq (ok_term_weaken_tvar empty_env)... }
-    Qed.
-
-    Lemma tm_ty_close_preservation :
-      forall Gamma t ty ty' k,
-        ok_term (BindTVar k :: Gamma) (tm_ty_open t 0 0) (ty_open ty 0 0) ->
-        ok_type Gamma ty' k ->
-        ok_term Gamma (tm_ty_bsubst t 0 ty') (ty_bsubst ty 0 ty').
-    Proof. Admitted.
 
   End Typing.
 End Typing.
